Problem when trying to use the mechanism on a piece of code

io/ho_examples/Callback.Example.fst
@@ -21,35 +21,60 @@ let pi cmd arg h =
     let fnm : io_args Openfile = arg in not (fnm = "/tmp/passwd")
   | _ -> true
 
-type cb_type   = fd:file_descr -> IIO bool         (fun h -> is_open fd h) (fun h _ lt -> lt == [])
-type f_type    = cb:cb_type    -> IIO (maybe unit) (fun _ -> True)            (fun h r lt -> enforced_locally pi h lt)
-type main_type = f: f_type     -> IIO unit         (fun _ -> True)            (fun h r lt -> enforced_locally pi h lt)
+unfold
+type cb  = fd:file_descr -> IIO (maybe bool) (fun h -> is_open fd h) (fun h _ lt -> lt == [])
+type ctx = cb:cb         -> IIO (maybe unit) (fun _ -> True)           (fun h r lt -> enforced_locally pi h lt)
+type pp  = f: ctx        -> IIO (maybe unit) (fun _ -> True)           (fun h r lt -> enforced_locally pi h lt)
 
-let cb_type_mlifyable : mlifyable cb_type = mlifyable_iiowp_post file_descr #(ML_FO mlfo_file_descr) bool #(ML_FO mlfo_bool) (fun fd h -> is_open fd h) (fun fd h _ lt -> lt == [])
+let cb_mlifyable : mlifyable cb = 
+  mlifyable_iiowp_trivialize_weaken_post
+    file_descr
+    bool
+    (fun fd h -> is_open fd h)
+    (fun fd h _ lt -> lt == [])
 
-let cb_type_mlifyable_guarded : mlifyable_guarded file_descr bool (fun fd h -> is_open fd h) (fun fd h r lt -> lt == []) pi = {
-  cmlifyable = cb_type_mlifyable;
-  cpi = ()
+let cb_mlifyable_guarded : mlifyable_guarded_arr1 file_descr bool (fun fd h -> is_open fd h) (fun fd h r lt -> lt == []) pi = {
+  ca1 = importable_safe_importable file_descr;
+  cmlifyable1 = cb_mlifyable;
+  cpi1 = ()
 }
 
 private
-let lemma_c1post () : squash (forall (x:cb_type_mlifyable_guarded.cmlifyable.matype) h lt. True /\ enforced_locally pi h lt ==> (exists (r:maybe unit). enforced_locally pi h lt)) by (explode (); witness (`(Inl ())))= ()
+let lemma_c1post () : squash (forall (x:cb_mlifyable_guarded.cmlifyable1.matype) h lt. True /\ enforced_locally pi h lt ==> (exists (r:maybe unit). enforced_locally pi h lt)) by (explode (); witness (`(Inl ())))= ()
 
 private
 let lemma_c2post () : squash (forall h lt. enforced_locally pi h lt  ==> enforced_locally pi h lt) =
   lemma_c1post ()
 
-let f_post_monitorable : monitorable_post (fun fd h -> True) (fun fd h r lt -> enforced_locally pi h lt) pi = {
+let pp_post_monitorable : monitorable_hist (fun fd h -> True) (fun fd h r lt -> enforced_locally pi h lt) pi = {
   result_check = (fun _ _ _ _ -> true);
   c1post = lemma_c1post ();
   c2post = lemma_c2post ();
 }
 
-let f_type_instrumentable : instrumentable f_type =
-  instrumentable_HO file_descr bool (fun fd h -> is_open fd h) (fun fd h r lt -> lt == []) unit (fun h -> True) (fun h r lt -> enforced_locally pi h lt) pi
+let ctx_instrumentable : instrumentable ctx pi =
+  instrumentable_HO_arr1_out_importable file_descr bool (fun fd h -> is_open fd h) (fun fd h r lt -> lt == []) unit (fun h -> True) (fun h r lt -> enforced_locally pi h lt) pi
   #(importable_safe_importable _ #(safe_importable_ml (maybe unit) #(mlfo_maybe unit #(ML_FO mlfo_unit))))
-  #cb_type_mlifyable_guarded
-  #f_post_monitorable
+  #cb_mlifyable_guarded
+  #pp_post_monitorable
   
-let main_mlifyable : mlifyable main_type =
-  mlifyable_inst_iiowp_post f_type unit (fun h r lt -> enforced_locally pi h lt) #f_type_instrumentable #(ML_FO mlfo_unit)
+let pp_mlifyable : mlifyable pp =
+  mlifyable_inst_iiowp_weaken ctx #ctx_instrumentable (maybe unit) (fun h r lt -> enforced_locally pi h lt)
+
+let main : pp = fun c ->
+  let theCb : cb = fun fd -> if is_open fd (get_trace ()) then Inl true else Inl false in
+  c theCb
+
+(** I can not write a context in the intermediate language because the type of the callback is not informative 
+    enough to know it respects pi. **)
+let c (theCb : file_descr -> MIIO (maybe bool)) : IIOpi (maybe unit) pi =
+  let fd = static_cmd Openfile "/tmp2/passwd" in
+  if Inl? fd  then
+    let test = theCb (Inl?.v fd) in
+    if Inl? test && Inl?.v test then Inl ()
+    else Inr Something_went_really_bad
+  else Inr Something_went_really_bad
+
+let main_mlify = mlify #_ #pp_mlifyable main
+
+let whole () : MIIO (maybe unit) = main_mlify c
